src/high/protocol.v
@@ -12,43 +12,47 @@ From self.high.modalities Require Import no_buffer.
 Definition loc_pred `{nvmG Σ} ST `{AbstractState ST} := ST → val → dProp Σ.
 
 (* A protocol consists of
-  - A predicate [pred] that holds for each write and corresponding state of the
+  - A predicate [p_inv] that holds for each write and corresponding state of the
     location.
   - A function [bumper] that specifies how the state of a location changes
     after a crash. *)
-Record LocationProtocol ST `{AbstractState ST, nvmG Σ} := {
-  pred : loc_pred ST;
-  bumper : ST → ST;
-  bumper_mono : Proper ((⊑@{ST}) ==> (⊑))%signature bumper;
-  pred_condition :
-    (⊢ ∀ s v, pred s v -∗ <PCF> pred (bumper s) v : dProp Σ)%I;
-  pred_nobuf :> ∀ s v, BufferFree (pred s v);
+Record LocationProtocol ST `{AbstractState ST, nvmG Σ} := MkProt {
+  p_inv : loc_pred ST;
+  p_bumper : ST → ST;
+  (* bumper_mono : Proper ((⊑@{ST}) ==> (⊑))%signature bumper; *)
+  (* pred_condition : *)
+  (*   (⊢ ∀ s v, p_inv s v -∗ <PCF> p_inv (bumper s) v : dProp Σ)%I; *)
+  (* pred_nobuf :> ∀ s v, BufferFree (p_inv s v); *)
 }.
 
-Global Arguments pred {ST} {_} {_} {_} {_} {_} _.
-Global Arguments bumper {ST} {_} {_} {_} {_} {_} _.
+Global Arguments p_inv {ST} {_} {_} {_} {_} {_} _.
+Global Arguments p_bumper {ST} {_} {_} {_} {_} {_} _.
+
+(* Type class collection the properties that a protocol should have.
+
+Note: The fields are ordered by "difficulty" in the sense of how difficult these
+conditions usually are to show.  *)
+Class ProtocolConditions `{AbstractState ST, nvmG Σ} (prot : LocationProtocol ST) := {
+  bumper_mono :
+    Proper ((⊑@{ST}) ==> (⊑))%signature (prot.(p_bumper));
+  inv_nobuf :>
+    ∀ s v, BufferFree (prot.(p_inv) s v);
+  pred_condition :
+    (⊢ ∀ s v, prot.(p_inv) s v -∗ <PCF> prot.(p_inv) (prot.(p_bumper) s) v : dProp Σ)%I;
+}.
+
+#[global] Hint Mode ProtocolConditions + + + + + + ! : typeclass_instances.
 
 Existing Instance bumper_mono.
-Existing Instance pred_nobuf.
-
-(* Creates a protocol with the [bumper] begin the identity function. *)
-Definition protocolIdBumper `{AbstractState ST, nvmG Σ}
-    (pred : loc_pred ST) pred_condition pred_nobuf :=
-  {|
-    pred := pred;
-    bumper := id;
-    bumper_mono := _;
-    pred_condition := pred_condition;
-    pred_nobuf := pred_nobuf;
-  |}.
+Existing Instance inv_nobuf.
 
 (** [know_protocol] represents the knowledge that a location is associated with a
 specific protocol. It's defined simply using more "primitive" assertions. *)
 Definition know_protocol `{AbstractState ST, nvmG Σ}
            ℓ (prot : LocationProtocol ST) : dProp Σ :=
-  "#knowPred" ∷ know_pred_d ℓ prot.(pred) ∗
+  "#knowPred" ∷ know_pred_d ℓ prot.(p_inv) ∗
   "#knowPreorder" ∷ know_preorder_loc_d ℓ (⊑@{ST}) ∗
-  "#knowBumper" ∷ know_bumper ℓ prot.(bumper).
+  "#knowBumper" ∷ know_bumper ℓ prot.(p_bumper).
 
 Lemma encode_bumper_bump_mono `{AbstractState ST}
       (bumper : ST → ST) `{!Proper ((⊑@{ST}) ==> (⊑))%signature bumper}
@@ -87,16 +91,16 @@ Section protocol.
 
   Lemma know_protocol_extract ℓ prot :
     know_protocol ℓ prot -∗
-      know_pred_d ℓ prot.(pred) ∗
+      know_pred_d ℓ prot.(p_inv) ∗
       know_preorder_loc_d ℓ (⊑@{ST}) ∗
-      know_bumper ℓ prot.(bumper).
+      know_bumper ℓ prot.(p_bumper).
   Proof. iNamed 1. iFrame "#". Qed.
 
   Lemma know_protocol_unfold ℓ prot i :
     know_protocol ℓ prot i ⊣⊢
-       ("#knowPred" ∷ know_pred_d ℓ (pred prot) i ∗
+       ("#knowPred" ∷ know_pred_d ℓ (p_inv prot) i ∗
         "#knowPreorder" ∷ know_preorder_loc_d ℓ (⊑@{ST}) i ∗
-        "#knowBumper" ∷ know_bumper ℓ (bumper prot) i).
+        "#knowBumper" ∷ know_bumper ℓ (p_bumper prot) i).
   Proof. rewrite /know_protocol !monPred_at_sep //. Qed.
 
   Global Instance know_protocol_buffer_free ℓ prot :
@@ -105,9 +109,9 @@ Section protocol.
 
   Lemma know_protocol_at ℓ prot TV gnames :
     (know_protocol ℓ prot) (TV, gnames) ⊣⊢
-      know_pred ℓ prot.(pred) ∗
+      know_pred ℓ prot.(p_inv) ∗
       know_preorder_loc ℓ (⊑@{ST}) ∗
-      own_know_bumper (get_bumpers_name gnames) ℓ prot.(bumper).
+      own_know_bumper (get_bumpers_name gnames) ℓ prot.(p_bumper).
   Proof.
     rewrite /know_protocol. rewrite !monPred_at_sep.
     simpl. rewrite !monPred_at_embed.
